verify/Bouncer2x5v1.v
@@ -1,0 +1,271 @@
+From BusyCoq Require Import Individual25.
+Require Import ZifyNat Lia.
+Require Import ZArith.
+Require Import String.
+Require Import List.
+
+
+Definition if_None {A} (a:option A) b :=
+match a with
+| None => b tt
+| _ => a
+end.
+
+Notation "a ||| b" := (if_None a b) (at level 30, right associativity).
+
+Import Eqb.
+
+Ltac des_if H :=
+  cbn[if_None] in H;
+  cbn[if_Some] in H;
+  let E:=fresh "E" in
+  match type of H with
+  | ?a ||| _ = _ =>
+    destruct a eqn:E
+  | ?a &&& _ = _ =>
+    destruct a eqn:E
+  end.
+
+Ltac crefl := vm_compute; try reflexivity.
+
+Ltac esc :=
+  (apply BoundedConfig.segRLs_c_spec with (T:=10^3); reflexivity) ||
+  (apply BoundedConfig.sideRLs_c_spec with (T:=10^3); reflexivity) ||
+  (eapply sideRLs_c_spec with (T:=10^6); [vm_compute; reflexivity | st; reflexivity]).
+
+Module TM1.
+Definition tm := Eval compute in (TM_from_str "1RB2LA0LB1LA2RA_0LA3RA1RA4LB---").
+Notation "c -->* c'" := (c -[ tm ]->* c') (at level 40).
+Notation "c -->+ c'" := (c -[ tm ]->+ c') (at level 40).
+
+Notation lh0 := (0inf<*<[1;3;1;3;3;2;3;3;1;3;1;3;1;3;3]).
+Notation lh1 := (0inf<*<[1;3;1;3;3;2;3;2;3;3;1;3;3;1;1;3;1;3;3;1;1;3;1;3;1;3;3]).
+Notation lh2 := (0inf<*<[1;3;1;3;3;2;3;3;1;3;1;3;3;1;1;2;1;3;3;1;1;3;3;1;1;3;1;3;3;1;1;3;1;3;1;3;3]).
+Notation w := [2;2;2;1;2;2;1;1;2;2;1;2;1;1;2;2;1;2;1;2;1;1;1;2;1;1;2;2;1;2;1;1;2;1].
+Notation hL := (A,[1;2;1;1;2;2;1;2;1;1;2;1]).
+Notation hR := (B,<[2;3;2;1;3;1]).
+Notation h := [(hR,hL)].
+
+Inductive Tp := tp0|tp1|tp2.
+
+Lemma w_Incs n:
+  segRLs tm h h (w^^n) (w^^n).
+Proof.
+  induction n.
+  1: esc.
+  cbn[lpow].
+  eapply segRLs_concat; eauto 1.
+  esc.
+Qed.
+
+Section maxT_sec.
+Hypothesis maxT:nat.
+Definition RInc0 r := sideRL_c tm hR hL r maxT.
+Definition RInc1 r := sideRL_c tm hR hL (w*>r) maxT.
+Definition MInc '(n,r) :=
+(RInc0 r &&& (fun r => Some (n,r))) ||| (fun _ =>
+match n with
+| O => None
+| S n => RInc1 r &&& (fun r => Some (n,r))
+end).
+
+Definition Inc '(n,r,tp) :=
+let '(n,tp) :=
+match tp with
+| tp0 => (n,tp1)
+| tp1 => (n,tp2)
+| tp2 => (S n,tp0)
+end in
+MInc (n,r) &&& (fun '(n,r) => Some (n,r,tp)).
+
+Lemma MInc_spec n r n' r':
+  MInc (n,r) = Some (n',r') ->
+  sideRLs tm h (w^^n *> r) (w^^n' *> r').
+Proof.
+  unfold MInc,RInc0,RInc1.
+  intros H.
+  des_if H.
+  - inverts H.
+    des_if E; inverts E.
+    eapply sideRL_c_spec in E0.
+    eapply segRLs_sideRLs_concat.
+    1: apply w_Incs.
+    econstructor; [apply E0| constructor].
+  - cbn[if_None] in H.
+    destruct n; [inverts H|].
+    des_if H; [|inverts H].
+    inverts H.
+    eapply sideRL_c_spec in E0.
+    replace (S n') with (n'+1) by lia.
+    rewrite <-lpow_add'.
+    eapply segRLs_sideRLs_concat.
+    1: apply w_Incs.
+    econstructor; [apply E0| constructor].
+Qed.
+
+Definition LC tp :=
+match tp with
+| tp0 => lh0
+| tp1 => lh1
+| tp2 => lh2
+end.
+
+Definition S' '(n,r,tp) := LC tp {{{ (hL,L) }}} w^^n *> r.
+
+Lemma Inc_spec x x':
+  Inc x = Some x' ->
+  S' x -->+ S' x'.
+Proof.
+  unfold S',LC,Inc.
+  destruct x as [[n r] tp].
+  destruct x' as [[n' r'] tp'].
+  intros.
+  destruct tp.
+  - des_if H. 2: inverts H.
+    destruct p as [n0 r0].
+    apply MInc_spec in E.
+    mid01 (lh1 {{{ (hR,R) }}} w^^n *> r).
+    1: es.
+    inverts H.
+    inverts E.
+    inverts H5.
+    apply H4.
+  - des_if H. 2: inverts H.
+    destruct p as [n0 r0].
+    apply MInc_spec in E.
+    mid01 (lh2 {{{ (hR,R) }}} w^^n *> r).
+    1: es.
+    inverts H.
+    inverts E.
+    inverts H5.
+    apply H4.
+  - des_if H. 2: inverts H.
+    destruct p as [n0 r0].
+    apply MInc_spec in E.
+    mid01 (lh0 {{{ (hR,R) }}} w^^(S n) *> r).
+    1: es.
+    inverts H.
+    inverts E.
+    inverts H5.
+    apply H4.
+Time Qed.
+
+Fixpoint Incs T x :=
+match T with
+| O => Some x
+| S T => Inc x &&& (fun x => Incs T x)
+end.
+
+Lemma Incs_spec T x x':
+  Incs T x = Some x' ->
+  S' x -->* S' x'.
+Proof.
+  gen x x'.
+  induction T; cbn; intros.
+  - inverts H.
+    finish.
+  - des_if H; inverts H.
+    apply Inc_spec in E.
+    apply IHT in H1.
+    eapply progress_evstep in E.
+    follow E.
+    apply H1.
+Qed.
+
+Lemma Incs_spec' T x x':
+  Incs (S T) x = Some x' ->
+  S' x -->+ S' x'.
+Proof.
+  cbn.
+  intros.
+  des_if H; inverts H.
+  apply Inc_spec in E.
+  follow10 E.
+  eapply Incs_spec,H1.
+Qed.
+
+Definition tp_eqb(a b:Tp):bool :=
+match a,b with
+| tp0,tp0 => true
+| tp1,tp1 => true
+| tp2,tp2 => true
+| _,_ => false
+end.
+
+Lemma tp_eqb_spec a b:
+  Bool.reflect (a=b) (tp_eqb a b).
+Proof.
+  destruct a,b; solve_Bool_reflect.
+Qed.
+
+Definition check_loop n0 r0 PP P PP' x :=
+  Incs PP x &&& (fun '(n,r,tp) =>
+  let r1:=Str_firstn PP' r in
+  Incs (S P) (n+n0,r1 *> r0,tp) &&& (fun '(n',r',tp') =>
+  if eqb r1 (Str_firstn PP' r') then
+  if Nat.leb n n' then
+  if tp_eqb tp tp' then Some tt
+  else None
+  else None
+  else None
+  )).
+
+Local Opaque Eqb.eqb Incs.
+
+Lemma check_loop_spec PP P PP' x:
+  (forall n0 r0,
+  check_loop n0 r0 PP P PP' x = Some tt) ->
+  ~halts tm (S' x).
+Proof.
+  unfold check_loop.
+  intros.
+  destruct (Incs PP x) as [[[n r] tp]|] eqn:E; cbn in H.
+  2: specialize (H O (const s0)); congruence.
+  eapply Incs_spec in E.
+  pose (fun '(n0,r0) => S' (n+n0,Str_firstn PP' r *> r0, tp)) as S''.
+  eapply multistep_nonhalt with (c':=S'' (O,Str_nth_tl PP' r)).
+  - unfold S''.
+    rewrite Nat.add_0_r.
+    rewrite <-Str_firstn_spec.
+    apply E.
+  - eapply progress_nonhalt_simple.
+    intros [n0 r0].
+    specialize (H n0 r0).
+    des_if H.
+    2: inverts H.
+    cbn in H.
+    destruct p as [[n' r'] tp'].
+    destruct (eqb_spec (Str_firstn PP' r) (Str_firstn PP' r')).
+    2: congruence.
+    destruct (Nat.leb_spec n n').
+    2: congruence.
+    destruct (tp_eqb_spec tp tp').
+    2: congruence.
+    subst.
+    eapply Incs_spec' in E0.
+    unfold S''.
+    exists (n'-n,Str_nth_tl PP' r').
+    follow10 E0.
+    rewrite e.
+    rewrite <-Str_firstn_spec.
+    finish.
+Qed.
+
+End maxT_sec.
+
+Ltac stepn n0 :=
+  eapply without_counter with (n:=N.to_nat n0);
+  eapply multistep_c_spec; vm_compute; try reflexivity.
+
+Lemma nonhalt: ~halts tm c0.
+Proof.
+  eapply multistep_nonhalt with (c':=S' (2%nat,_,tp0)).
+  1: stepn 115664%N.
+  eapply check_loop_spec with (maxT:=10^6) (PP:=110000) (P:=78506*3-1) (PP':=21866).
+  intros.
+  native_check_eq.
+Time Qed.
+
+End TM1.
+
+
