verify/SOMDC2x5v2.v
@@ -1,0 +1,338 @@
+From BusyCoq Require Import Individual25 DivModCases.
+Require Import ZifyNat Lia.
+Require Import ZArith.
+Require Import String.
+Require Import List.
+
+Lemma segRLs_addmul_v2 a a' x b b' tm h w1 w2:
+  segRLs tm (h^^b) (h^^b') w1 w2 ->
+  segRLs tm (h^^a) (h^^a') w2 w2 ->
+  segRLs tm (h^^(x*a+b)) (h^^(x*a'+b')) w1 w2.
+Proof.
+  intros.
+  rewrite (Nat.add_comm _ b).
+  rewrite (Nat.add_comm _ b').
+  do 2 rewrite lpow_add.
+  eapply segRLs_trans.
+  1: apply H.
+  induction x; cbn[Nat.mul].
+  - cbn.
+    constructor.
+  - cbn[lpow].
+    do 2 rewrite lpow_add.
+    eapply segRLs_trans.
+    2: apply IHx.
+    apply H0.
+Qed.
+
+
+Ltac esc :=
+  (apply BoundedConfig.segRLs_c_spec with (T:=10^3); reflexivity) ||
+  (apply BoundedConfig.sideRLs_c_spec with (T:=10^3); reflexivity) ||
+  (eapply sideRLs_c_spec with (T:=10^6); [vm_compute; reflexivity | st; reflexivity]).
+
+Module TM1.
+Definition tm := Eval compute in (TM_from_str "1RB4LA1LB2LA0RB_2LB3RB4LA---1RA").
+Notation "c -->* c'" := (c -[ tm ]->* c') (at level 40).
+Notation "c -->+ c'" := (c -[ tm ]->+ c') (at level 40).
+
+Notation hR := (B,<[]).
+Notation hR' := (A,<[1]).
+Notation hL := (A,[]).
+Notation h := [(hR,hL)].
+Notation h' := [(hR',hL)].
+
+Notation ld := [4;4].
+Notation d0 := [2;2].
+Notation d1 := [4;2].
+
+Lemma ld_Incs k:
+  segRLs tm (h^^k) (h^^(k*2)) ld ld.
+Proof.
+  applys_eq (segRLs_addmul_v2 1 2 k 0 0); unfold DH0.
+  1,2: flia.
+  1,2: esc.
+Qed.
+
+Lemma d00_Incs k:
+  segRLs tm (h^^(k*2)) (h^^k) d0 d0.
+Proof.
+  applys_eq (segRLs_addmul_v2 2 1 k 0 0); unfold DH0.
+  1,2: flia.
+  1,2: esc.
+Qed.
+
+Lemma d01_Incs k:
+  segRLs tm (h^^(1+k*2)) (h^^k) d0 d1.
+Proof.
+  applys_eq (segRLs_addmul_v2 2 1 k 1 0); unfold DH0.
+  1,2: flia.
+  1,2: esc.
+Qed.
+
+Notation rh := ([4;2;4]*>0inf).
+
+Inductive RD := D0|D1|LD.
+
+Fixpoint toRC ls :=
+match ls with
+| [] => rh
+| D0::t => d0 *> toRC t
+| D1::t => d1 *> toRC t
+| LD::t => ld *> toRC t
+end.
+
+Inductive RC: nat->(list RD)->Prop :=
+| RC_0: RC O []
+| RC_1 k r: RC k r -> RC (1+k*2) (D0::r)
+| RC_2 k r: RC k r -> RC (2+k*2) (D1::r).
+
+Ltac ec := econstructor.
+
+Lemma RC_ex k:
+  exists r, RC k r.
+Proof.
+  induction k using lt_wf_ind; intros.
+  destruct (mod2 k); subst.
+  - destruct a.
+    + ec; ec.
+    + unshelve epose proof (H a _) as [r I1].
+      1: lia.
+      ec; ec; apply I1.
+  - unshelve epose proof (H a _) as [r I1].
+    1: lia.
+    ec; ec; apply I1.
+Qed.
+
+Lemma RC_spec k r:
+  RC k r ->
+  sideRLs tm (h^^k) rh (toRC r).
+Proof.
+  gen r.
+  induction k using lt_wf_ind; intros.
+  assert ((k=0 \/ k=1+k/2*2 \/ k=2+(k/2-1)*2)%nat) as [E|[E|E]] by lia.
+  - subst.
+    inverts H0.
+    esc.
+  - inverts H0; try lia.
+    rewrite lpow_add.
+    eapply @sideRLs_trans with (r2:=d0*>rh).
+    1: esc.
+    eapply segRLs_sideRLs_concat.
+    1: apply d00_Incs.
+    eapply H; eauto 1; lia.
+  - inverts H0; try lia.
+    change (2+k0*2) with (1+(1+k0*2)).
+    rewrite lpow_add.
+    eapply @sideRLs_trans with (r2:=d0*>rh).
+    1: esc.
+    eapply segRLs_sideRLs_concat.
+    1: apply d01_Incs.
+    eapply H; eauto 1; lia.
+Qed.
+
+Inductive RIncs: nat->(list RD)->(list RD)->Prop :=
+| RIncs_O k r:
+  RC (k*4) r ->
+  RIncs (1+k) [] (LD::LD::r)
+| RIncs_ld k r r':
+  RIncs (1+k*2) r r' ->
+  RIncs k (LD::r) (LD::r')
+| RIncs_d1 k r r':
+  RIncs (k*2) r r' ->
+  RIncs k (D1::r) (LD::r')
+| RIncs_d00 k r r':
+  RIncs k r r' ->
+  RIncs (2+k*2) (D0::r) (D0::r')
+| RIncs_d01 k r r':
+  RIncs k r r' ->
+  RIncs (3+k*2) (D0::r) (D1::r')
+.
+
+Lemma RIncs_spec k r r':
+  RIncs k r r' ->
+  sideRLs tm (h'++h^^k) (toRC r) (toRC r').
+Proof.
+  intro H.
+  induction H.
+  { rewrite lpow_add,app_assoc.
+    apply RC_spec in H.
+    eapply @sideRLs_trans with (r2:=ld*>ld*>rh).
+    1: esc.
+    eapply segRLs_sideRLs_concat.
+    1: apply ld_Incs.
+    eapply segRLs_sideRLs_concat.
+    1: apply ld_Incs.
+    applys_eq H; flia. }
+  { eapply segRLs_sideRLs_concat; [|apply IHRIncs].
+    rewrite lpow_add,app_assoc.
+    eapply segRLs_trans.
+    2: apply ld_Incs.
+    esc. }
+  { eapply segRLs_sideRLs_concat; [|apply IHRIncs].
+    eapply segRLs_trans.
+    2: apply ld_Incs.
+    esc. }
+  { eapply segRLs_sideRLs_concat; [|apply IHRIncs].
+    rewrite lpow_add,app_assoc.
+    eapply segRLs_trans.
+    2: apply d00_Incs.
+    esc. }
+  { eapply segRLs_sideRLs_concat; [|apply IHRIncs].
+    change (3+k*2) with (2+(1+k*2)).
+    rewrite lpow_add,app_assoc.
+    eapply segRLs_trans.
+    2: apply d01_Incs.
+    esc. }
+Qed.
+
+Inductive full: nat->Prop :=
+| full_O: full 0
+| full_S k: full k -> full (1+k*2).
+
+Inductive notfull: nat->Prop :=
+| notfull_0 k: full k -> notfull (2+k*2)
+| notfull_1 k: notfull k -> notfull (1+k*2)
+| notfull_2 k: notfull k -> notfull (2+k*2)
+.
+
+Lemma notfull_ge2 [k]:
+  notfull k ->
+  2<=k.
+Proof.
+  intro H.
+  induction H; lia.
+Qed.
+
+Lemma RC_RIncs_full [k r k']:
+  RC k r ->
+  1+k*3<=k' ->
+  full k ->
+  exists r', RIncs k' r r'.
+Proof.
+  intro H.
+  gen k'.
+  induction H; intros.
+  - destruct (sub k' 1); [subst|lia].
+    epose proof (RC_ex _) as [r I1].
+    ec; ec; apply I1.
+  - inverts H1.
+    replace k0 with k in * by lia.
+    destruct (sub k' 2); [subst|lia].
+    destruct (mod2 c); subst.
+    + epose proof (IHRC a _ H3) as [r' I1].
+      ec; ec; apply I1.
+    + epose proof (IHRC a _ H3) as [r' I1].
+      ec; ec; apply I1.
+  - inverts H1; lia.
+  Unshelve. all: lia.
+Qed.
+
+
+Lemma RC_RIncs_notfull [k r k']:
+  RC k r ->
+  k<=1+k' ->
+  notfull k ->
+  exists r', RIncs k' r r'.
+Proof.
+  intro H.
+  gen k'.
+  induction H; intros.
+  - inverts H0.
+  - inverts H1; try lia.
+    replace k0 with k in * by lia.
+    epose proof (notfull_ge2 H3).
+    destruct (sub k' 2); [subst|lia].
+    destruct (mod2 c); subst.
+    + epose proof (IHRC a _ H3) as [r' I1].
+      ec; ec; apply I1.
+    + epose proof (IHRC a _ H3) as [r' I1].
+      ec; ec; apply I1.
+  - inverts H1; try lia.
+    + replace k0 with k in * by lia.
+      eapply (RC_RIncs_full) with (k':=k'*2) in H; eauto 1.
+      2: lia.
+      destruct H as [r' I1].
+      ec; ec; apply I1.
+    + replace k0 with k in * by lia.
+      epose proof (IHRC (k'*2) _ H3) as [r' I1].
+      ec; ec; apply I1.
+  Unshelve. all: lia.
+Qed.
+
+Lemma RC_full_cases [k r]:
+  RC k r ->
+  full k \/ notfull k.
+Proof.
+  intro H.
+  induction H.
+  - left; ec.
+  - destruct IHRC as [I|I]; (left+right); ec; apply I.
+  - destruct IHRC as [I|I]; (left+right); ec; apply I.
+Qed.
+
+Lemma RIncs_nxt k r r':
+  RIncs k r r' ->
+  forall k',
+  k<=k' ->
+  exists r'',
+  RIncs k' r' r''.
+Proof.
+  intros H.
+  induction H; intros. 
+  - destruct (RC_full_cases H) as [I|I].
+    + pose proof I as I0.
+      inverts I0; try lia.
+      epose proof (RC_RIncs_full H _ I) as [r' I1].
+      do 3 ec; apply I1.
+    + epose proof (RC_RIncs_notfull H _ I) as [r' I1].
+      do 3 ec; apply I1.
+  - epose proof (IHRIncs (1+k'*2) _) as [r'' I1].
+    ec; ec; apply I1.
+  - epose proof (IHRIncs (1+k'*2) _) as [r'' I1].
+    ec; ec; apply I1.
+  - destruct (sub k' 2); [subst|lia].
+    destruct (mod2 c); subst.
+    + epose proof (IHRIncs a _) as [r'' I1].
+      ec; ec; apply I1.
+    + epose proof (IHRIncs a _) as [r'' I1].
+      ec; ec; apply I1.
+  - epose proof (IHRIncs (k'*2) _) as [r'' I1].
+    ec; ec; apply I1.
+  Unshelve. all: try lia.
+Qed.
+
+Notation lh := (0inf<*[1]).
+Definition S' r := lh {{{ (hR',R) }}} toRC r.
+
+Lemma BigStep r r':
+  RIncs 0 r r' ->
+  S' r -->+
+  S' r'.
+Proof.
+  intro H.
+  apply RIncs_spec in H.
+  unfold S'.
+  epose proof (sideRLs_concat (sideRLseq_O _ _) H) as I1.
+  follow10 I1.
+  er.
+Qed.
+
+Lemma nonhalt: ~halts tm c0.
+Proof.
+  eapply multistep_nonhalt with (c':=S' [LD;LD;LD;D1;D1]).
+  1: er.
+  eapply progress_nonhalt_cond with (P:=fun r => exists r', RIncs 0 r r').
+  2:{
+    epose proof (RC_ex _) as [r' I1].
+    eexists.
+    do 6 ec; apply I1.
+  }
+  intros r [r' I1].
+  exists r'; split.
+  - apply BigStep,I1.
+  - eapply RIncs_nxt; eauto 1.
+Qed.
+
+End TM1.
+
